\textbf{Time Complexity Determination}: Express the time complexity of the following program fragment as a 
Big-Theta asymptotic, in terms of $n$. You must also prove that your answer is correct.

\begin{algorithm}
    \SetAlgoLined
    % \DontPrintSemicolon
    \For{$i \gets 1$ \KwTo $n$}{\;  
    \For{$j \gets 1$ \KwTo $i$}{\; 
        \For{$k \gets 1$ \KwTo $j$}{\;
            $s \gets s + i - j \cdot k$\;  
        }
    }
}
\end{algorithm}
\begin{customsolutionbox}
    Time complexity is $\Theta(n^3)$. We see that for each $k$, $s \gets s + i - j \cdot k$ has $\Theta(1)$ which 
    executed $j$ times for $j^{th}$ iteration of the second loop.
    \begin{align}
        T(n) &=  \sum_{i=1}^{n} \sum_{j=1}^{i} \Theta(1) \cdot j \\
        &= \sum_{i=1}^{n} \Theta\left(\frac{i^2 + i}{2}\right)\\
        &= \frac{1}{2}\left(\sum_{i=1}^{n} \Theta(i^2)+\sum_{i=1}^{n}  \Theta(i)\right)\\
        &= \frac{1}{2} \cdot\left(\frac{n(n+1)(2n+1)}{6}+ \frac{n(n+1)}{2}\right) \\
        &= \left(\frac{2n^3+3n^2+n}{12}\right) + \left(\frac{n^2+n}{4}\right) \\
        &=  \frac{2n^3+3n^2+n+3n^2+3n}{12} \\
        &=  \frac{2n^3+6n^2+4n}{12} \\
    \end{align}
    To see that $T(n) = \mathcal{O}(n^3)$, we can see that:
    \begin{align}
        T(n) &= \frac{2n^3+6n^2+4n}{12} \\
        &\leq  \frac{2n^3+6n^3+4n^3}{12} \\
        &= \frac{12}{12} \cdot n^3 \\
        &= n^3
    \end{align}
    Therefore, $T(n) = \mathcal{O}(n^3)$ for some $n_0$ and $c$ such that $n_0 = 1$ and $c = 1$. \\
    To see that $T(n) = \Omega(n^3)$, we can see that:
    \begin{align}
        T(n) &= \frac{2n^3+6n^2+4n}{12} \\
        &\geq  \frac{2n^3}{12} \\
        &= \frac{1}{6} n^3
    \end{align}
    Therefore, $T(n) = \Omega(n^3)$ for some $n_0$ and $c$ such that $n_0 = 1$ and $c = \frac{1}{6}$, hence
    $T(n) = \Theta(n^3)$. \\
\end{customsolutionbox}